fix CI WIP
src/Main.fst fails...
likely need to split it

src/StarMalloc.fst
@@ -248,7 +248,7 @@ let full_getsize (ptr: array U8.t)
       (G.reveal (snd result) ==> (
         let idx = sc_selection (US.sizet_to_uint32 (fst result)) in
         (enable_sc_fast_selection ==>
-          A.length ptr == U32.v (L.index sc_list (US.v idx))) /\
+          A.length ptr == U32.v (get_u32 (L.index sc_list (US.v idx)))) /\
         (enable_slab_canaries_malloc ==>
           A.length ptr == US.v (fst result) + 2
         ) /\
@@ -292,7 +292,7 @@ let getsize (ptr: array U8.t)
       (US.v result <= U32.v page_size ==> (
         let idx = sc_selection (US.sizet_to_uint32 result) in
         (enable_sc_fast_selection ==>
-          A.length ptr == U32.v (L.index sc_list (US.v idx))) /\
+          A.length ptr == U32.v (get_u32 (L.index sc_list (US.v idx)))) /\
         (enable_slab_canaries_malloc ==>
           A.length ptr == US.v result + 2
         ) /\
@@ -319,7 +319,7 @@ let realloc_small_optim_lemma
     US.v old_size <= U32.v page_size /\
     US.v new_size <= US.v threshold /\
     (let old_idx = sc_selection (US.sizet_to_uint32 old_size) in
-    let old_sc = L.index sc_list (US.v old_idx) in
+    let old_sc = get_u32 (L.index sc_list (US.v old_idx)) in
     let new_idx = if enable_slab_canaries_malloc
       then sc_selection (US.sizet_to_uint32 (US.add new_size 2sz))
       else sc_selection (US.sizet_to_uint32 new_size) in
