src/Main.fst
@@ -1103,6 +1103,8 @@ let init_wrapper2 sc n k k' slab_region md_bm_region md_region
 module G = FStar.Ghost
 module UP = FStar.PtrdiffT
 
+#restart-solver
+
 #push-options "--fuel 0 --ifuel 0 --z3rlimit 50"
 let slab_region_size
   : v:US.t{
@@ -3293,7 +3295,7 @@ let init_one_arena2
 
 #restart-solver
 
-#push-options "--fuel 0 --ifuel 0 --z3rlimit 500 --split_queries no --query_stats"
+#push-options "--fuel 0 --ifuel 0 --z3rlimit 800 --split_queries no --query_stats"
 noextract inline_for_extraction
 val init_nth_arena_aux
   (l1:list sc)
@@ -3433,10 +3435,6 @@ val init_nth_arena_aux
 #restart-solver
 
 let _ = ()
-
-#restart-solver
-
-#restart-solver
 
 #push-options "--fuel 0 --ifuel 0 --z3rlimit 800 --query_stats"
 //--z3cliopt smt.arith.nl=false"
